$f(x,t) = $ $\prod_{i=0}^{t-1}(x + i) $ ,求 $\sum_{x=1}^nf(x,s)$,答案对$10^9+7$ 取模， $n \le 10^{18},s \le 2 \times 10^5$        [I-小 S 的数学题](https://ac.nowcoder.com/acm/contest/95480/I)



$ \prod_{i=0}^{s-1}(x+i) =$   $\{$ $ \prod_{i=0}^{s}(x+i) -$ $ \prod_{i=-1}^{s-1}(x+i) $ $\}$   $\div$  $（s + 1）$   

  $x \cdot(x+1)\cdot(x+2) \cdot\cdot\cdot (x+s-1) \times(s+1) =$  $x \cdot(x+1)\cdot(x+2) \cdot\cdot\cdot (x+s) - $  $(x-1) \cdot(x)\cdot(x+1) \cdot\cdot\cdot (x+s-1)$  

​                                                                                       $\Rightarrow$  $\{$ $x \cdot(x+1)\cdot(x+2) \cdot\cdot\cdot (x+s-1)$   $\}$    $\times$ $\{$  $(x+s) - (x-1)$  $\}$  

$\sum_{x=1}^nf(x,s) = $ $\sum_{x=1}^{n} \prod_{i=0}^{s-1}(x+i)$  

​						  $ =$   $\frac{ \prod_{i=0}^{s}(x+i) -\prod_{i=-1}^{s-1}(x+i)}{s+1}$

令$f(x) = \prod_{i=0}^s(x+i)$ , $g(x) = \prod_{i=-1}^{s-1}(x+i)$ 

$f(1) = \prod_{i=0}^s(1+i)$ ,$g(2) = \prod_{i=-1}^{s-1}(2+i) = f(1)$ 

$\sum_{x=1}^nf(x,s) = $ $\frac{f(1) -  g(1) + f(2) - g(2) + f(3) - g(3) +\cdot\cdot\cdot + f(n) - g(n)}{s+1} = $  $\frac{f(n) - g(1)}{s+1}$    且$g(1) = 0$      

$Ans=$$\frac{f(n)}{s+1}$ ,对$10^9+7$ 取模   

```c++

void solve() {
    ll n,s;
    std::cin >> n >> s;
    ll ans = n;	
    ans %= mod;
    for(int i = 1; i <= s; i++) {
    	ans = ans * ((i + n) % mod);
    	ans %= mod;
    }
    ans = ans * ksm(s + 1,mod - 2) % mod;
    std::cout << ans << '\n';
    return;
}
```

